src/ReactorModel/Determinism/ChangeListEquiv.lean
@@ -2,10 +2,10 @@ import ReactorModel.Execution
 
 open Classical
 
-structure ChangeListEquiv (cs₁ cs₂ : List Change) : Prop where
-  ports   : ∀ i,   cs₁.lastSome? (·.portValue? i)     = cs₂.lastSome? (·.portValue? i)
-  state   : ∀ i,   cs₁.lastSome? (·.stateValue? i)    = cs₂.lastSome? (·.stateValue? i)
-  actions : ∀ i t, cs₁.filterMap (·.actionValue? i t) = cs₂.filterMap (·.actionValue? i t)
+structure ChangeListEquiv (cs₁ cs₂ : List (Identified Change)) : Prop where
+  ports   : ∀ i,   cs₁.lastSome? (·.obj.portValue? i)     = cs₂.lastSome? (·.obj.portValue? i)
+  state   : ∀ i,   cs₁.lastSome? (·.obj.stateValue? i)    = cs₂.lastSome? (·.obj.stateValue? i)
+  actions : ∀ i t, cs₁.filterMap (·.obj.actionValue? i t) = cs₂.filterMap (·.obj.actionValue? i t)
   -- NOTE: Mutations are currently noops, and can therefore be ignored.
 
 notation cs₁:max " ⋈ " cs₂:max => ChangeListEquiv cs₁ cs₂
