src/ReactorModel/Determinism/InstExecution.lean
@@ -4,12 +4,12 @@ open Classical
 
 namespace Execution
 
-theorem InstExecution.preserves_tag : (s₁ ⇓ᵢ+[rcns] s₂) → s₁.ctx.tag = s₂.ctx.tag
+theorem InstExecution.preserves_tag : (s₁ ⇓ᵢ+ s₂) → s₁.ctx.tag = s₂.ctx.tag
   | single h => h.preserves_tag
   | trans h hi => h.preserves_tag.trans hi.preserves_tag
 
-theorem InstExecution.preserves_ctx_past_future {s₁ s₂ rcns} :
-  (s₁ ⇓ᵢ+[rcns] s₂) → ∀ g, g ≠ s₁.ctx.tag → s₁.ctx.processedRcns g = s₂.ctx.processedRcns g := by
+theorem InstExecution.preserves_ctx_past_future {s₁ s₂} :
+  (s₁ ⇓ᵢ+ s₂) → ∀ g, g ≠ s₁.ctx.tag → s₁.ctx.processedRcns g = s₂.ctx.processedRcns g := by
   intro h g hg
   induction h
   case single h => exact h.preserves_ctx_past_future _ hg
@@ -18,12 +18,12 @@ theorem InstExecution.preserves_ctx_past_future {s₁ s₂ rcns} :
     exact (he.preserves_ctx_past_future _ hg).trans $ hi hg
     
 theorem InstExecution.preserves_rcns {i : ID} :
-  (s₁ ⇓ᵢ+[rcns] s₂) → (s₁.rtr.obj? .rcn i = s₂.rtr.obj? .rcn i)
+  (s₁ ⇓ᵢ+ s₂) → (s₁.rtr.obj? .rcn i = s₂.rtr.obj? .rcn i)
   | single h => h.preserves_rcns
   | trans h₁ₘ hₘ₂ => h₁ₘ.preserves_rcns.trans hₘ₂.preserves_rcns
 
 theorem InstExecution.rcns_unprocessed : 
-  (s₁ ⇓ᵢ+[rcns] s₂) → ∀ rcn ∈ rcns, rcn ∉ s₁.ctx.currentProcessedRcns := by
+  (e : s₁ ⇓ᵢ+ s₂) → ∀ rcn ∈ e.rcns, rcn ∉ s₁.ctx.currentProcessedRcns := by
   intro h rcn hr
   induction h
   case single h => simp [List.mem_singleton.mp hr, h.rcn_unprocessed]
@@ -34,12 +34,12 @@ theorem InstExecution.rcns_unprocessed :
       specialize hi h
       exact ((not_or _ _).mp $ (mt h₁.mem_currentProcessedRcns.mpr) hi).right
 
-theorem InstExecution.rcns_nodup : (s₁ ⇓ᵢ+[rcns] s₂) → List.Nodup rcns
+theorem InstExecution.rcns_nodup : (e : s₁ ⇓ᵢ+ s₂) → List.Nodup e.rcns
   | single _ => List.nodup_singleton _
   | trans h₁ h₂ => List.nodup_cons.mpr $ ⟨(mt $ h₂.rcns_unprocessed _) $ not_not.mpr h₁.self_currentProcessedRcns, h₂.rcns_nodup⟩
 
 theorem InstExecution.currentProcessedRcns_monotonic :
-  (s₁ ⇓ᵢ+[rcns] s₂) → s₁.ctx.currentProcessedRcns ⊆ s₂.ctx.currentProcessedRcns := by
+  (s₁ ⇓ᵢ+ s₂) → s₁.ctx.currentProcessedRcns ⊆ s₂.ctx.currentProcessedRcns := by
   intro h
   apply Finset.subset_iff.mpr
   intro rcn hr
@@ -48,34 +48,34 @@ theorem InstExecution.currentProcessedRcns_monotonic :
   case trans h _ hi => exact hi $ h.monotonic_currentProcessedRcns hr
 
 theorem InstExecution.mem_currentProcessedRcns :
-  (s₁ ⇓ᵢ+[rcns] s₂) → ∀ rcn, rcn ∈ s₂.ctx.currentProcessedRcns ↔ rcn ∈ rcns ∨ rcn ∈ s₁.ctx.currentProcessedRcns := by
+  (e : s₁ ⇓ᵢ+ s₂) → ∀ rcn, rcn ∈ s₂.ctx.currentProcessedRcns ↔ rcn ∈ e.rcns ∨ rcn ∈ s₁.ctx.currentProcessedRcns := by
   intro h rcn
   induction h
-  case single h => simp [List.mem_singleton, h.mem_currentProcessedRcns]
-  case trans hd _ tl _ h₁ _ hi => 
+  case single h => simp [rcns, List.mem_singleton, h.mem_currentProcessedRcns]
+  case trans h₁ h₂ hi => 
     constructor <;> intro hc 
     case mp =>
       cases hi.mp hc with
       | inl h => exact .inl $ List.mem_cons_of_mem _ h
       | inr h => 
-        by_cases hc : rcn ∈ (hd::tl)
+        by_cases hc : rcn ∈ (h₁.rcn :: h₂.rcns)
         case pos => exact .inl hc
         case neg => exact .inr $ (h₁.mem_currentProcessedRcns.mp h).resolve_left $ List.ne_of_not_mem_cons hc
     case mpr =>
       cases hc with
       | inl h => 
         cases (List.mem_cons_iff ..).mp h with
-        | inl h => rw [←h] at h₁; exact hi.mpr $ .inr h₁.self_currentProcessedRcns
+        | inl h => exact hi.mpr $ .inr (h ▸ h₁.self_currentProcessedRcns)
         | inr h => exact hi.mpr $ .inl h
       | inr h => exact hi.mpr $ .inr $ h₁.monotonic_currentProcessedRcns h
 
 -- Corollary of `InstExecution.mem_currentProcessedRcns`.
 theorem InstExecution.self_currentProcessedRcns : 
-  (s₁ ⇓ᵢ+[rcns] s₂) → ∀ rcn ∈ rcns, rcn ∈ s₂.ctx.currentProcessedRcns := 
+  (e : s₁ ⇓ᵢ+ s₂) → ∀ rcn ∈ e.rcns, rcn ∈ s₂.ctx.currentProcessedRcns := 
   λ h _ hm => (h.mem_currentProcessedRcns _).mpr $ .inl hm
   
 theorem InstExecution.eq_ctx_processed_rcns_perm : 
-  (s ⇓ᵢ+[rcns₁] s₁) → (s ⇓ᵢ+[rcns₂] s₂) → (s₁.ctx = s₂.ctx) → rcns₁ ~ rcns₂ := by
+  (e₁ : s ⇓ᵢ+ s₁) → (e₂ : s ⇓ᵢ+ s₂) → (s₁.ctx = s₂.ctx) → e₁.rcns ~ e₂.rcns := by
   intro h₁ h₂ he
   apply (List.perm_ext h₁.rcns_nodup h₂.rcns_nodup).mpr
   intro rcn
@@ -96,71 +96,38 @@ theorem InstExecution.eq_ctx_processed_rcns_perm :
       exact ((h₁.mem_currentProcessedRcns _).mp h).resolve_right hc
 
 theorem InstExecution.rcns_respect_dependencies : 
-  (s₁ ⇓ᵢ+[rcns] s₂) →
-  rcns.get? i₁ = some rcn₁ → rcns.get? i₂ = some rcn₂ → 
+  (e : s₁ ⇓ᵢ+ s₂) →
+  e.rcns.get? i₁ = some rcn₁ → e.rcns.get? i₂ = some rcn₂ → 
   rcn₁ >[s₁.rtr] rcn₂ → i₁ < i₂ := by
   intro h h₁ h₂ hd
   sorry
 
-theorem InstExecution.rcn_list_cons : (s₁ ⇓ᵢ+[rcns] s₂) → ∃ hd tl, rcns = hd :: tl :=
-  (by cases · <;> simp)
+theorem InstExecution.rcn_list_cons : (e : s₁ ⇓ᵢ+ s₂) → ∃ hd tl, e.rcns = hd :: tl :=
+  (by cases · <;> simp [rcns])
 
--- A Given list of change segments is well-formed over a given instantaneous execution,
--- if each set of changes corresponds to the output of the reaction at the same position. 
-inductive InstExecution.Changes.WFSegments : (s₁ ⇓ᵢ+[rcns] s₂) → List (List Change) → Prop
-  | singleSkip (e : s₁ ⇓ᵢ[rcn] s₂) : (s₁.rcnOutput rcn = none)    → WFSegments (.single e) [[]]
-  | singleExec (e : s₁ ⇓ᵢ[rcn] s₂) : (s₁.rcnOutput rcn = some cs) → WFSegments (.single e) [cs]
-  | transSkip (e₁ : s₁ ⇓ᵢ[hd] s') {e₂ : s' ⇓ᵢ+[tl] s₂} : (s₁.rcnOutput hd = none) → (WFSegments e₂ ctl) → WFSegments (.trans e₁ e₂) ctl
-  | transExec (e₁ : s₁ ⇓ᵢ[hd] s') {e₂ : s' ⇓ᵢ+[tl] s₂} : (s₁.rcnOutput hd = some chd) → (WFSegments e₂ ctl) → WFSegments (.trans e₁ e₂) ([chd] ++ ctl)
-
--- This structure flattens an instantaneous execution into a list of changes.
-structure InstExecution.Changes (h : s₁ ⇓ᵢ+[rcns] s₂) where
-  segments : List (List Change)
-  endState : State
-  wfExec : ∃ rcn, s₁ -[rcn:segments.join]→* endState -- The `∃ rcn` is kind of weird, but hopefully we'll remove the whole lifting of reactions into the execution relations at some point - then this can be dropped.
-  wfEndState : s₂ = { endState with ctx := endState.ctx.addCurrentProcessed' rcns }
-  wfSegments : Changes.WFSegments h segments
-
-theorem InstExecution.Changes.intro : (h : s₁ ⇓ᵢ+[rcns] s₂) → Nonempty (InstExecution.Changes h) := by
-  intro h
-  induction h
-  case single h =>
-    have ⟨cs, s₂', _, h₁, h₂⟩ := h.changes
-    refine Nonempty.intro ?_
-    apply Changes.mk [cs] s₂'
-    case wfExec => simp; exact ⟨_, h₁⟩
-    case wfEndState => exact h₂
-    case wfSegments =>
-      cases H : h
-      case execReaction =>
-        apply Changes.WFSegments.singleExec h 
-        sorry
-      all_goals sorry
-  case trans hd s₂ tl s₃ hhd htl hi =>
-    -- have ⟨tlcs, tls₂', _, _⟩ := hi
-    -- have ⟨hdcs, _, _, h₁, h₂⟩ := hhd.changes
-    -- exists [hdcs] ++ tlcs
-    sorry
-    -- i think we can' prove the rest here because we're missing the execution contexts.
-    -- figure out a nice way (perhaps a structure) to state the property that should be the result of this theorem.
-    -- that would probably also help you with proving it.
-
+theorem InstExecution.to_ChangeListStep :
+  (e : s₁ ⇓ᵢ+ s₂) → (s₁ -[e.changes]→* ⟨s₂.rtr, s₁.ctx⟩) := by
+  intro e
+  induction e
+  case single e => simp [changes, e.to_ChangeListStep]
+  case trans s₁ sₘ s₂ e₁ e₂ hi => 
+    have h := e₁.to_ChangeListStep
+    simp [changes]
+    have hs := ChangeListStep.append h hi rfl
+    exact hs
+  
 -- This theorem is the main theorem about determinism in an instantaneous setting.
 -- Basically, if the same reactions have been executed, then we have the same resulting
 -- reactor.
 protected theorem InstExecution.deterministic : 
-  (s ⇓ᵢ+[rcns₁] s₁) → (s ⇓ᵢ+[rcns₂] s₂) → (s₁.ctx = s₂.ctx) → s₁ = s₂ := by
+  (s ⇓ᵢ+ s₁) → (s ⇓ᵢ+ s₂) → (s₁.ctx = s₂.ctx) → s₁ = s₂ := by
   intro h₁ h₂ hc
   refine State.ext _ _ ?_ hc
   have hp := h₁.eq_ctx_processed_rcns_perm h₂ hc
-  let cs₁ := Changes.intro h₁ |>.some
-  let cs₂ := Changes.intro h₂ |>.some
-  suffices h : cs₁.segments.join ⋈ cs₂.segments.join by 
-    have h' := cs₁.wfExec.choose_spec.equiv_changes_eq_result cs₂.wfExec.choose_spec h
-    have h₁ : cs₁.endState.rtr = s₁.rtr := by simp [cs₁.wfEndState]
-    have h₂ : cs₂.endState.rtr = s₂.rtr := by simp [cs₂.wfEndState]
-    simp [←h₁, ←h₂, h']
-  sorry -- TODO: This is the next big theorem.
+  suffices h : h₁.changes ⋈ h₂.changes by 
+    injection h₁.to_ChangeListStep.equiv_changes_eq_result h₂.to_ChangeListStep h
+    assumption
+  sorry
     
     
       
