src/ReactorModel/Execution/Context.lean
@@ -33,6 +33,10 @@ noncomputable def addCurrentProcessed' (ctx : Context) : List ID → Context
   | [] => ctx
   | hd :: tl => (ctx.addCurrentProcessed hd).addCurrentProcessed' tl
 
+theorem addCurrentProcessed'_singleton (ctx : Context) :
+  ctx.addCurrentProcessed' [i] = ctx.addCurrentProcessed i :=
+  sorry  
+
 theorem addCurrentProcessed_preserves_ctx_past_future (ctx : Context) (i : ID) : ∀ g, g ≠ ctx.tag → (ctx.addCurrentProcessed i).processedRcns g = ctx.processedRcns g := by
   intro g h
   simp [addCurrentProcessed, Finmap.update_ne _ h.symm]
